gravy/test/out.bpl
@@ -9,11 +9,21 @@ type intArrHeap_type = [ref][int]int;
 const unique $type : Field javaType;
 const unique $alloc : Field bool;
 const unique $null : ref;
-const { :sourceloc "a",-1,-1,-1,-1 } unique java.lang.Object : javaType extends  complete;
-const { :sourceloc "a",-1,-1,-1,-1 } unique TruePositive06 : javaType extends  unique java.lang.Object complete;
-const { :sourceloc "a",-1,-1,-1,-1 } unique java.io.Serializable : javaType extends  unique java.lang.Object complete;
-const { :sourceloc "a",-1,-1,-1,-1 } unique java.lang.Comparable : javaType extends  unique java.lang.Object complete;
-const { :sourceloc "a",-1,-1,-1,-1 } unique java.lang.Character : javaType extends  unique java.lang.Comparable, unique java.io.Serializable, unique java.lang.Object complete;
+const { :sourceloc "/Users/schaef/git/jar2bpl/jar2bpl_test/regression/false_positives/fp16/FalsePositive16.java",-1,-1,-1,-1 } unique java.lang.Object : javaType extends  complete;
+const { :sourceloc "/Users/schaef/git/jar2bpl/jar2bpl_test/regression/false_positives/fp16/FalsePositive16.java",-1,-1,-1,-1 } unique FalsePositive16 : javaType extends  unique java.lang.Object complete;
+const { :sourceloc "/Users/schaef/git/jar2bpl/jar2bpl_test/regression/false_positives/fp16/FalsePositive16.java",-1,-1,-1,-1 } unique java.io.Serializable : javaType extends  unique java.lang.Object complete;
+const { :sourceloc "/Users/schaef/git/jar2bpl/jar2bpl_test/regression/false_positives/fp16/FalsePositive16.java",-1,-1,-1,-1 } unique java.lang.Comparable : javaType extends  unique java.lang.Object complete;
+const { :sourceloc "/Users/schaef/git/jar2bpl/jar2bpl_test/regression/false_positives/fp16/FalsePositive16.java",-1,-1,-1,-1 } unique java.lang.CharSequence : javaType extends  unique java.lang.Object complete;
+const { :sourceloc "/Users/schaef/git/jar2bpl/jar2bpl_test/regression/false_positives/fp16/FalsePositive16.java",-1,-1,-1,-1 } unique java.lang.String : javaType extends  unique java.lang.CharSequence, unique java.lang.Comparable, unique java.io.Serializable, unique java.lang.Object complete;
+const { :sourceloc "/Users/schaef/git/jar2bpl/jar2bpl_test/regression/false_positives/fp16/FalsePositive16.java",-1,-1,-1,-1 } unique java.lang.Throwable : javaType extends  unique java.io.Serializable, unique java.lang.Object complete;
+const { :sourceloc "/Users/schaef/git/jar2bpl/jar2bpl_test/regression/false_positives/fp16/FalsePositive16.java",-1,-1,-1,-1 } unique java.lang.Exception : javaType extends  unique java.lang.Throwable complete;
+const unique $StringConst0 : ref extends  complete;
+const { :sourceloc "/Users/schaef/git/jar2bpl/jar2bpl_test/regression/false_positives/fp16/FalsePositive16.java",-1,-1,-1,-1 } unique java.lang.RuntimeException : javaType extends  unique java.lang.Exception complete;
+const { :sourceloc "/Users/schaef/git/jar2bpl/jar2bpl_test/regression/false_positives/fp16/FalsePositive16.java",-1,-1,-1,-1 } unique java.lang.NullPointerException : javaType extends  unique java.lang.RuntimeException complete;
+const { :sourceloc "/Users/schaef/git/jar2bpl/jar2bpl_test/regression/false_positives/fp16/FalsePositive16.java",-1,-1,-1,-1 } unique java.lang.IndexOutOfBoundsException : javaType extends  unique java.lang.RuntimeException complete;
+const { :sourceloc "/Users/schaef/git/jar2bpl/jar2bpl_test/regression/false_positives/fp16/FalsePositive16.java",-1,-1,-1,-1 } unique java.lang.ArrayIndexOutOfBoundsException : javaType extends  unique java.lang.IndexOutOfBoundsException complete;
+const unique $StringConst1 : ref extends  complete;
+const unique $LongConst0 : int extends  complete;
 var $heap : $heap_type;
 var $intArrayType : javaType;
 var $charArrayType : javaType;
@@ -42,95 +52,574 @@ function $shlInt(x:int, y:int) returns ($ret:int);
 function $ushrInt(x:int, y:int) returns ($ret:int);
 function $shrInt(x:int, y:int) returns ($ret:int);
 axiom (forall t : javaType :: $heap[$null,$type] <: t);
-procedure $new(obj_type:javaType) returns ($obj:ref);    ensures $obj != $null;    ensures $heap[$obj,$type] == obj_type;        ensures $heap[$obj,$alloc] == true;    requires $heap[$obj,$alloc] == false;
+procedure $new(obj_type:javaType) returns ($obj:ref);        ensures $heap[$obj,$alloc] == true;    requires $heap[$obj,$alloc] == false;    ensures $heap[$obj,$type] == obj_type;    ensures $obj != $null;
 
-procedure java.lang.Object$java.lang.Object$clone$43($this:ref) returns ($other:ref);    ensures $heap[$other,$alloc] == true;    ensures $heap[$other,$type] == $heap[$this,$type];    ensures $other != $null;    
+procedure java.lang.Object$java.lang.Object$clone$43($this:ref) returns ($other:ref);    ensures $heap[$other,$type] == $heap[$this,$type];    ensures $other != $null;    ensures $heap[$other,$alloc] == true;    
 
 procedure int$java.lang.String$compareTo$87($this:ref, $other:ref) returns ($return:int);    
 
-procedure int$TruePositive06$doubleLoop2$1889($this:ref) returns ($return:int, $exception:ref);    
+procedure void$FalsePositive16$sendMessage$1889($this:ref, $in_parameter__0:ref, $in_parameter__1:ref) returns ($exception:ref);    
 
-procedure void$TruePositive06$foo$1890($this:ref, $in_parameter__0:ref) returns ($exception:ref);    
+procedure java.lang.Object$FalsePositive16$getSender$1892($this:ref) returns ($return:ref, $exception:ref);    
 
-procedure void$java.lang.Character$$la$init$ra$$1621($this:ref, $in_parameter__0:int) returns ($exception:ref);    
+procedure void$java.lang.Exception$$la$init$ra$$628($this:ref, $in_parameter__0:ref) returns ($exception:ref);    
 
-procedure boolean$java.lang.Character$isLetterOrDigit$1668($in_parameter__0:int) returns ($return:int, $exception:ref);    
+procedure void$java.lang.NullPointerException$$la$init$ra$$1888($this:ref, $in_parameter__0:ref) returns ($exception:ref);    
 
-procedure void$TruePositive06$$la$init$ra$$1891($this:ref) returns ($exception:ref);    
+procedure void$FalsePositive16$addFaultyMember$1891($this:ref, $in_parameter__0:ref, $in_parameter__1:ref) returns ($exception:ref);    
+
+procedure int$java.lang.Object$hashCode$41($this:ref) returns ($return:int, $exception:ref);    
+
+procedure java.lang.String$java.lang.Object$toString$44($this:ref) returns ($return:ref, $exception:ref);    
+
+procedure void$FalsePositive16$returnSender$1890($this:ref, $in_parameter__0:ref) returns ($exception:ref);    
+
+procedure void$FalsePositive16$foo$1893($this:ref, $in_parameter__0:int) returns ($exception:ref);    
+
+procedure void$FalsePositive16$decideCondition$1894($this:ref, $in_parameter__0:int, $in_parameter__1:int) returns ($exception:ref);    
+
+procedure void$java.lang.RuntimeException$$la$init$ra$$922($this:ref) returns ($exception:ref);    
+
+procedure int$FalsePositive16$decisions$1895($this:ref, $in_parameter__0:int, $in_parameter__1:int) returns ($return:int, $exception:ref);    
+
+procedure void$FalsePositive16$$la$init$ra$$1896($this:ref) returns ($exception:ref);    
 
 procedure void$java.lang.Object$$la$init$ra$$38($this:ref) returns ($exception:ref);    
 
-implementation int$TruePositive06$doubleLoop2$1889($this:ref) returns ($return:int, $exception:ref){
+implementation void$FalsePositive16$sendMessage$1889($this:ref, $in_parameter__0:ref, $in_parameter__1:ref) returns ($exception:ref){
     
-var temp$05 : int;    
-var temp$38 : int;    
-var j4 : int;    
+var temp$1118 : ref;    
+var temp$613 : ref;    
+var i8 : int;    
+var temp$29 : int;    
 var this1 : ref;    
-var temp$16 : int;    
-var i3 : int;    
-var ret2 : int;    
-var temp$510 : int;    
-var temp$27 : int;    
-var temp$49 : int;
-    assume { :sourceloc "a",-1,-1,-1,-1 } $this != $null;
-    assert { :sourceloc "a",6,2,15,2 } true;
+var temp$714 : int;    
+var cx6 : ref;    
+var $fakelocal_1 : ref;    
+var temp$815 : int;    
+var $fakelocal_2 : int;    
+var destination2 : ref;    
+var msg3 : ref;    
+var sender4 : ref;    
+var temp$05 : ref;    
+var temp$512 : ref;    
+var temp$17 : ref;    
+var $fakelocal_3 : ref;    
+var $fakelocal_0 : ref;    
+var temp$411 : int;    
+var temp$310 : ref;
+    assume { :sourceloc "/Users/schaef/git/jar2bpl/jar2bpl_test/regression/false_positives/fp16/FalsePositive16.java",-1,-1,-1,-1 } $this != $null;
+    assume $heap[$in_parameter__1,$type] <: java.lang.String;
+    assert { :sourceloc "/Users/schaef/git/jar2bpl/jar2bpl_test/regression/false_positives/fp16/FalsePositive16.java",13,2,32,2 } true;
     this1 := $this;
-    assert { :sourceloc "a",7,9,7,18 } true;
-    ret2 := 0;
-    assert { :sourceloc "a",8,14,8,20 } true;
-    i3 := 0;
+    assert { :sourceloc "/Users/schaef/git/jar2bpl/jar2bpl_test/regression/false_positives/fp16/FalsePositive16.java",13,26,13,45 } true;
+    destination2 := $in_parameter__0;
+    assert { :sourceloc "/Users/schaef/git/jar2bpl/jar2bpl_test/regression/false_positives/fp16/FalsePositive16.java",13,48,13,57 } true;
+    msg3 := $in_parameter__1;
+    assert { :sourceloc "/Users/schaef/git/jar2bpl/jar2bpl_test/regression/false_positives/fp16/FalsePositive16.java",14,3,14,23 } true;
+    sender4 := $null;
   block1:
-    assert { :sourceloc "a",8,23,8,26 } true;
-    if (i3 < 10) {
-        assert { :sourceloc "a",8,23,8,26 } { :comment "thenblock" } true;
-        goto block2;
-    } else {
-        assert { :sourceloc "a",8,23,8,26 } { :comment "elseblock" } true;
+    assert { :sourceloc "/Users/schaef/git/jar2bpl/jar2bpl_test/regression/false_positives/fp16/FalsePositive16.java",16,13,16,23 } true;
+    call temp$05, $exception := java.lang.Object$FalsePositive16$getSender$1892(this1);
+    if ($exception != $null) {
+        if ($heap[$exception,$type] <: java.lang.Throwable) {
+            assert { :clone } true;
+            goto block2;
+        } else {
+            assert { :clone } true;
+        }
     }
-    assert { :sourceloc "a",8,23,8,26 } true;
-    goto block3;
-  block2:
-    assert { :sourceloc "a",10,18,10,24 } true;
-    j4 := 0;
-  block4:
-    assert { :sourceloc "a",10,27,10,30 } true;
-    if (j4 < 10) {
-        assert { :sourceloc "a",10,27,10,30 } { :comment "thenblock" } true;
-        goto block5;
+    assert { :sourceloc "/Users/schaef/git/jar2bpl/jar2bpl_test/regression/false_positives/fp16/FalsePositive16.java",16,4,16,9 } true;
+    sender4 := temp$05;
+    assert { :sourceloc "/Users/schaef/git/jar2bpl/jar2bpl_test/regression/false_positives/fp16/FalsePositive16.java",17,8,17,21 } true;
+    if (sender4 == $null) {
+        assert { :sourceloc "/Users/schaef/git/jar2bpl/jar2bpl_test/regression/false_positives/fp16/FalsePositive16.java",17,8,17,21 } { :clone } { :comment "thenblock" } true;
+        goto block3;
     } else {
-        assert { :sourceloc "a",10,27,10,30 } { :comment "elseblock" } true;
+        assert { :sourceloc "/Users/schaef/git/jar2bpl/jar2bpl_test/regression/false_positives/fp16/FalsePositive16.java",17,8,17,21 } { :clone } { :comment "elseblock" } true;
     }
-    assert { :sourceloc "a",10,27,10,30 } true;
-    goto block6;
-  block5:
-    assert { :sourceloc "a",11,17,11,22 } true;
-    temp$05 := ret2;
-    assert { :sourceloc "a",11,17,11,19 } true;
-    temp$16 := temp$05 + 1;
-    assert { :sourceloc "a",11,17,11,19 } true;
-    ret2 := temp$16;
-    assert { :sourceloc "a",10,33,10,35 } true;
-    temp$27 := i3;
-    assert { :sourceloc "a",10,33,10,33 } true;
-    temp$38 := temp$27 + 1;
-    assert { :sourceloc "a",10,33,10,33 } true;
-    i3 := temp$38;
-    assert { :sourceloc "a",10,13,12,13 } true;
+    assert { :sourceloc "/Users/schaef/git/jar2bpl/jar2bpl_test/regression/false_positives/fp16/FalsePositive16.java",17,8,17,21 } true;
     goto block4;
-  block6:
-    assert { :sourceloc "a",8,29,8,31 } true;
-    temp$49 := i3;
-    assert { :sourceloc "a",8,29,8,29 } true;
-    temp$510 := temp$49 + 1;
-    assert { :sourceloc "a",8,29,8,29 } true;
-    i3 := temp$510;
-    assert { :sourceloc "a",8,9,13,9 } true;
-    goto block1;
   block3:
-    assert { :sourceloc "a",14,4,14,14 } true;
-    $return := ret2;
+    assert { :sourceloc "/Users/schaef/git/jar2bpl/jar2bpl_test/regression/false_positives/fp16/FalsePositive16.java",18,5,19,65 } true;
+    call $fakelocal_0 := $new(java.lang.Exception);
+    temp$17 := $fakelocal_0;
+    assert { :sourceloc "/Users/schaef/git/jar2bpl/jar2bpl_test/regression/false_positives/fp16/FalsePositive16.java",18,20,19,64 } true;
+    call $exception := void$java.lang.Exception$$la$init$ra$$628(temp$17, $StringConst0);
+    if ($exception != $null) {
+        temp$17 := $null;
+        if ($heap[$exception,$type] <: java.lang.Throwable) {
+            assert { :clone } true;
+            goto block2;
+        } else {
+            assert { :clone } true;
+        }
+    }
+    assert { :sourceloc "/Users/schaef/git/jar2bpl/jar2bpl_test/regression/false_positives/fp16/FalsePositive16.java",18,20,19,64 } true;
+    cx6 := temp$17;
+    assert { :sourceloc "/Users/schaef/git/jar2bpl/jar2bpl_test/regression/false_positives/fp16/FalsePositive16.java",20,10,20,18 } true;
+    i8 := 0;
+  block5:
+    assert { :sourceloc "/Users/schaef/git/jar2bpl/jar2bpl_test/regression/false_positives/fp16/FalsePositive16.java",20,21,20,42 } true;
+    if (destination2 != $null) {
+        assert { :sourceloc "/Users/schaef/git/jar2bpl/jar2bpl_test/regression/false_positives/fp16/FalsePositive16.java",20,21,20,42 } true;
+    } else {
+        assert { :sourceloc "/Users/schaef/git/jar2bpl/jar2bpl_test/regression/false_positives/fp16/FalsePositive16.java",20,21,20,42 } true;
+        assert { :noverify } true;
+        call $exception := $new(java.lang.NullPointerException);
+        goto block2;
+    }
+    temp$29 := $arrSizeHeap[destination2];
+    assert { :sourceloc "/Users/schaef/git/jar2bpl/jar2bpl_test/regression/false_positives/fp16/FalsePositive16.java",20,21,20,42 } true;
+    if (i8 < temp$29) {
+        assert { :sourceloc "/Users/schaef/git/jar2bpl/jar2bpl_test/regression/false_positives/fp16/FalsePositive16.java",20,21,20,42 } { :comment "thenblock" } true;
+        goto block6;
+    } else {
+        assert { :sourceloc "/Users/schaef/git/jar2bpl/jar2bpl_test/regression/false_positives/fp16/FalsePositive16.java",20,21,20,42 } { :comment "elseblock" } true;
+    }
+    assert { :sourceloc "/Users/schaef/git/jar2bpl/jar2bpl_test/regression/false_positives/fp16/FalsePositive16.java",20,21,20,42 } true;
+    goto block7;
+  block6:
+    assert { :sourceloc "/Users/schaef/git/jar2bpl/jar2bpl_test/regression/false_positives/fp16/FalsePositive16.java",21,6,22,59 } true;
+    temp$310 := destination2;
+    assert { :sourceloc "/Users/schaef/git/jar2bpl/jar2bpl_test/regression/false_positives/fp16/FalsePositive16.java",21,6,22,59 } true;
+    temp$411 := i8;
+    assert { :sourceloc "/Users/schaef/git/jar2bpl/jar2bpl_test/regression/false_positives/fp16/FalsePositive16.java",21,6,22,59 } true;
+    if (temp$411 < $arrSizeHeap[temp$310] && temp$411 >= 0) {
+        assert { :sourceloc "/Users/schaef/git/jar2bpl/jar2bpl_test/regression/false_positives/fp16/FalsePositive16.java",21,6,22,59 } true;
+    } else {
+        assert { :sourceloc "/Users/schaef/git/jar2bpl/jar2bpl_test/regression/false_positives/fp16/FalsePositive16.java",21,6,22,59 } true;
+        assert { :noverify } true;
+        call $exception := $new(java.lang.ArrayIndexOutOfBoundsException);
+        goto block2;
+    }
+    temp$512 := $refArrHeap[temp$310][temp$411];
+    assert { :sourceloc "/Users/schaef/git/jar2bpl/jar2bpl_test/regression/false_positives/fp16/FalsePositive16.java",21,6,22,59 } true;
+    call $fakelocal_1 := $new(java.lang.NullPointerException);
+    temp$613 := $fakelocal_1;
+    assert { :sourceloc "/Users/schaef/git/jar2bpl/jar2bpl_test/regression/false_positives/fp16/FalsePositive16.java",21,38,22,58 } true;
+    call $exception := void$java.lang.NullPointerException$$la$init$ra$$1888(temp$613, $StringConst1);
+    if ($exception != $null) {
+        temp$613 := $null;
+        if ($heap[$exception,$type] <: java.lang.Throwable) {
+            assert { :clone } true;
+            goto block2;
+        } else {
+            assert { :clone } true;
+        }
+    }
+    assert { :sourceloc "/Users/schaef/git/jar2bpl/jar2bpl_test/regression/false_positives/fp16/FalsePositive16.java",21,38,22,58 } true;
+    call $exception := void$FalsePositive16$addFaultyMember$1891(this1, temp$512, temp$613);
+    if ($exception != $null) {
+        if ($heap[$exception,$type] <: java.lang.Throwable) {
+            assert { :clone } true;
+            goto block2;
+        } else {
+            assert { :clone } true;
+        }
+    }
+    assert { :sourceloc "/Users/schaef/git/jar2bpl/jar2bpl_test/regression/false_positives/fp16/FalsePositive16.java",20,45,20,47 } true;
+    temp$714 := i8;
+    assert { :sourceloc "/Users/schaef/git/jar2bpl/jar2bpl_test/regression/false_positives/fp16/FalsePositive16.java",20,45,20,45 } true;
+    temp$815 := temp$714 + 1;
+    assert { :sourceloc "/Users/schaef/git/jar2bpl/jar2bpl_test/regression/false_positives/fp16/FalsePositive16.java",20,45,20,45 } true;
+    i8 := temp$815;
+    assert { :sourceloc "/Users/schaef/git/jar2bpl/jar2bpl_test/regression/false_positives/fp16/FalsePositive16.java",20,5,22,60 } true;
+    goto block5;
+  block7:
+    assert { :sourceloc "/Users/schaef/git/jar2bpl/jar2bpl_test/regression/false_positives/fp16/FalsePositive16.java",23,5,23,13 } true;
+    $exception := cx6;
+    goto block2;
+  block4:
+    assert { :sourceloc "/Users/schaef/git/jar2bpl/jar2bpl_test/regression/false_positives/fp16/FalsePositive16.java",25,5,25,22 } true;
+    call $fakelocal_2, $exception := int$java.lang.Object$hashCode$41(sender4);
+    if ($exception != $null) {
+        if ($heap[$exception,$type] <: java.lang.Throwable) {
+            assert { :clone } true;
+            goto block2;
+        } else {
+            assert { :clone } true;
+        }
+    }
+    assert { :sourceloc "/Users/schaef/git/jar2bpl/jar2bpl_test/regression/false_positives/fp16/FalsePositive16.java",27,4,27,21 } true;
+    call $fakelocal_3, $exception := java.lang.String$java.lang.Object$toString$44(sender4);
+    if ($exception != $null) {
+        if ($heap[$exception,$type] <: java.lang.Throwable) {
+            assert { :clone } true;
+            goto block2;
+        } else {
+            assert { :clone } true;
+        }
+    }
+    assert { :sourceloc "/Users/schaef/git/jar2bpl/jar2bpl_test/regression/false_positives/fp16/FalsePositive16.java",29,8,29,21 } { :clone } true;
+    if (sender4 != $null) {
+        assert { :sourceloc "/Users/schaef/git/jar2bpl/jar2bpl_test/regression/false_positives/fp16/FalsePositive16.java",29,8,29,21 } { :clone } { :comment "thenblock" } true;
+        goto block8;
+    } else {
+        assert { :sourceloc "/Users/schaef/git/jar2bpl/jar2bpl_test/regression/false_positives/fp16/FalsePositive16.java",29,8,29,21 } { :clone } { :comment "elseblock" } true;
+    }
+    assert { :sourceloc "/Users/schaef/git/jar2bpl/jar2bpl_test/regression/false_positives/fp16/FalsePositive16.java",29,8,29,21 } { :clone } true;
+    goto block9;
+  block8:
+    assert { :sourceloc "/Users/schaef/git/jar2bpl/jar2bpl_test/regression/false_positives/fp16/FalsePositive16.java",30,5,30,24 } { :clone } true;
+    call $exception := void$FalsePositive16$returnSender$1890(this1, sender4);
+    if ($exception != $null) {
+        if ($heap[$exception,$type] <: java.lang.Throwable) {
+            assert { :clone } true;
+            goto block2;
+        } else {
+            assert { :clone } true;
+        }
+    }
+  block9:
+    assert { :sourceloc "/Users/schaef/git/jar2bpl/jar2bpl_test/regression/false_positives/fp16/FalsePositive16.java",15,3,31,3 } true;
+    goto block10;
+  block2:
+    assert { :sourceloc "/Users/schaef/git/jar2bpl/jar2bpl_test/regression/false_positives/fp16/FalsePositive16.java",15,3,31,3 } true;
+    assume $heap[$exception,$type] <: java.lang.Throwable;
+    temp$1118 := $exception;
+    assert { :sourceloc "/Users/schaef/git/jar2bpl/jar2bpl_test/regression/false_positives/fp16/FalsePositive16.java",29,8,29,21 } { :clone } true;
+    if (sender4 != $null) {
+        assert { :sourceloc "/Users/schaef/git/jar2bpl/jar2bpl_test/regression/false_positives/fp16/FalsePositive16.java",29,8,29,21 } { :clone } { :comment "thenblock" } true;
+        goto block11;
+    } else {
+        assert { :sourceloc "/Users/schaef/git/jar2bpl/jar2bpl_test/regression/false_positives/fp16/FalsePositive16.java",29,8,29,21 } { :clone } { :comment "elseblock" } true;
+    }
+    assert { :sourceloc "/Users/schaef/git/jar2bpl/jar2bpl_test/regression/false_positives/fp16/FalsePositive16.java",29,8,29,21 } { :clone } true;
+    goto block12;
+  block11:
+    assert { :sourceloc "/Users/schaef/git/jar2bpl/jar2bpl_test/regression/false_positives/fp16/FalsePositive16.java",30,5,30,24 } { :clone } true;
+    assert { :sourceloc "/Users/schaef/git/jar2bpl/jar2bpl_test/regression/false_positives/fp16/FalsePositive16.java",30,5,30,24 } { :clone } this1 != $null;
+    call $exception := void$FalsePositive16$returnSender$1890(this1, sender4);
+  block12:
+    assert { :sourceloc "/Users/schaef/git/jar2bpl/jar2bpl_test/regression/false_positives/fp16/FalsePositive16.java",30,5,30,24 } { :clone } true;
+    $exception := temp$1118;
+    return;
+  block10:
+    assert { :sourceloc "/Users/schaef/git/jar2bpl/jar2bpl_test/regression/false_positives/fp16/FalsePositive16.java",28,5,31,3 } true;
     return;
 }
 
+
+implementation void$FalsePositive16$returnSender$1890($this:ref, $in_parameter__0:ref) returns ($exception:ref){
+    
+var sender20 : ref;    
+var this19 : ref;
+    assume { :sourceloc "/Users/schaef/git/jar2bpl/jar2bpl_test/regression/false_positives/fp16/FalsePositive16.java",-1,-1,-1,-1 } $this != $null;
+    assume $heap[$in_parameter__0,$type] <: java.lang.Object;
+    assert { :sourceloc "/Users/schaef/git/jar2bpl/jar2bpl_test/regression/false_positives/fp16/FalsePositive16.java",34,2,37,2 } true;
+    this19 := $this;
+    assert { :sourceloc "/Users/schaef/git/jar2bpl/jar2bpl_test/regression/false_positives/fp16/FalsePositive16.java",34,28,34,40 } true;
+    sender20 := $in_parameter__0;
+    assert { :sourceloc "/Users/schaef/git/jar2bpl/jar2bpl_test/regression/false_positives/fp16/FalsePositive16.java",34,28,34,40 } true;
+    return;
+}
+
+
+implementation void$FalsePositive16$addFaultyMember$1891($this:ref, $in_parameter__0:ref, $in_parameter__1:ref) returns ($exception:ref){
+    
+var object22 : ref;    
+var nullPointerException23 : ref;    
+var this21 : ref;
+    assume { :sourceloc "/Users/schaef/git/jar2bpl/jar2bpl_test/regression/false_positives/fp16/FalsePositive16.java",-1,-1,-1,-1 } $this != $null;
+    assume $heap[$in_parameter__0,$type] <: java.lang.Object;
+    assume $heap[$in_parameter__1,$type] <: java.lang.NullPointerException;
+    assert { :sourceloc "/Users/schaef/git/jar2bpl/jar2bpl_test/regression/false_positives/fp16/FalsePositive16.java",39,2,43,2 } true;
+    this21 := $this;
+    assert { :sourceloc "/Users/schaef/git/jar2bpl/jar2bpl_test/regression/false_positives/fp16/FalsePositive16.java",39,31,39,43 } true;
+    object22 := $in_parameter__0;
+    assert { :sourceloc "/Users/schaef/git/jar2bpl/jar2bpl_test/regression/false_positives/fp16/FalsePositive16.java",40,4,40,44 } true;
+    nullPointerException23 := $in_parameter__1;
+    assert { :sourceloc "/Users/schaef/git/jar2bpl/jar2bpl_test/regression/false_positives/fp16/FalsePositive16.java",40,4,40,44 } true;
+    return;
+}
+
+
+implementation java.lang.Object$FalsePositive16$getSender$1892($this:ref) returns ($return:ref, $exception:ref){
+    
+var temp$025 : ref;    
+var this24 : ref;
+    assume { :sourceloc "/Users/schaef/git/jar2bpl/jar2bpl_test/regression/false_positives/fp16/FalsePositive16.java",-1,-1,-1,-1 } $this != $null;
+    assume $heap[$return,$type] <: java.lang.Object;
+    assert { :sourceloc "/Users/schaef/git/jar2bpl/jar2bpl_test/regression/false_positives/fp16/FalsePositive16.java",45,2,48,2 } true;
+    this24 := $this;
+    assert { :sourceloc "/Users/schaef/git/jar2bpl/jar2bpl_test/regression/false_positives/fp16/FalsePositive16.java",45,2,48,2 } true;
+    temp$025 := $null;
+    assert { :sourceloc "/Users/schaef/git/jar2bpl/jar2bpl_test/regression/false_positives/fp16/FalsePositive16.java",47,3,47,14 } true;
+    $return := temp$025;
+    return;
+}
+
+
+implementation void$FalsePositive16$foo$1893($this:ref, $in_parameter__0:int) returns ($exception:ref){
+    
+var temp$028 : int;    
+var temp$129 : int;    
+var this26 : ref;    
+var available27 : int;
+    assume { :sourceloc "/Users/schaef/git/jar2bpl/jar2bpl_test/regression/false_positives/fp16/FalsePositive16.java",-1,-1,-1,-1 } $this != $null;
+    assert { :sourceloc "/Users/schaef/git/jar2bpl/jar2bpl_test/regression/false_positives/fp16/FalsePositive16.java",55,2,59,2 } true;
+    this26 := $this;
+    assert { :sourceloc "/Users/schaef/git/jar2bpl/jar2bpl_test/regression/false_positives/fp16/FalsePositive16.java",55,18,55,31 } true;
+    available27 := $in_parameter__0;
+    assert { :sourceloc "/Users/schaef/git/jar2bpl/jar2bpl_test/regression/false_positives/fp16/FalsePositive16.java",56,8,56,21 } true;
+    temp$028 := $cmpInt(available27, 0);
+    assert { :sourceloc "/Users/schaef/git/jar2bpl/jar2bpl_test/regression/false_positives/fp16/FalsePositive16.java",56,8,56,21 } true;
+    if (temp$028 <= 0) {
+        assert { :sourceloc "/Users/schaef/git/jar2bpl/jar2bpl_test/regression/false_positives/fp16/FalsePositive16.java",56,8,56,21 } { :comment "thenblock" } true;
+        goto block13;
+    } else {
+        assert { :sourceloc "/Users/schaef/git/jar2bpl/jar2bpl_test/regression/false_positives/fp16/FalsePositive16.java",56,8,56,21 } { :comment "elseblock" } true;
+    }
+    assert { :sourceloc "/Users/schaef/git/jar2bpl/jar2bpl_test/regression/false_positives/fp16/FalsePositive16.java",56,8,56,21 } true;
+    goto block14;
+  block14:
+    assert { :sourceloc "/Users/schaef/git/jar2bpl/jar2bpl_test/regression/false_positives/fp16/FalsePositive16.java",56,28,56,53 } true;
+    temp$129 := $cmpInt(available27, $LongConst0);
+    assert { :sourceloc "/Users/schaef/git/jar2bpl/jar2bpl_test/regression/false_positives/fp16/FalsePositive16.java",56,28,56,53 } true;
+    if (temp$129 >= 0) {
+        assert { :sourceloc "/Users/schaef/git/jar2bpl/jar2bpl_test/regression/false_positives/fp16/FalsePositive16.java",56,28,56,53 } { :comment "thenblock" } true;
+        goto block13;
+    } else {
+        assert { :sourceloc "/Users/schaef/git/jar2bpl/jar2bpl_test/regression/false_positives/fp16/FalsePositive16.java",56,28,56,53 } { :comment "elseblock" } true;
+    }
+    assert { :sourceloc "/Users/schaef/git/jar2bpl/jar2bpl_test/regression/false_positives/fp16/FalsePositive16.java",56,28,56,53 } true;
+    goto block13;
+  block13:
+    assert { :sourceloc "/Users/schaef/git/jar2bpl/jar2bpl_test/regression/false_positives/fp16/FalsePositive16.java",57,4,57,12 } true;
+    return;
+}
+
+
+implementation void$FalsePositive16$decideCondition$1894($this:ref, $in_parameter__0:int, $in_parameter__1:int) returns ($exception:ref){
+    
+var this31 : ref;    
+var truthValue32 : int;    
+var $fakelocal_0 : ref;    
+var temp$034 : ref;    
+var notEqual33 : int;
+    assume { :sourceloc "/Users/schaef/git/jar2bpl/jar2bpl_test/regression/false_positives/fp16/FalsePositive16.java",-1,-1,-1,-1 } $this != $null;
+    assert { :sourceloc "/Users/schaef/git/jar2bpl/jar2bpl_test/regression/false_positives/fp16/FalsePositive16.java",64,2,79,2 } true;
+    this31 := $this;
+    assert { :sourceloc "/Users/schaef/git/jar2bpl/jar2bpl_test/regression/false_positives/fp16/FalsePositive16.java",64,30,64,43 } true;
+    truthValue32 := $in_parameter__0;
+    assert { :sourceloc "/Users/schaef/git/jar2bpl/jar2bpl_test/regression/false_positives/fp16/FalsePositive16.java",64,46,64,61 } true;
+    notEqual33 := $in_parameter__1;
+    assert { :sourceloc "/Users/schaef/git/jar2bpl/jar2bpl_test/regression/false_positives/fp16/FalsePositive16.java",68,7,68,14 } true;
+    if (notEqual33 == 0) {
+        assert { :sourceloc "/Users/schaef/git/jar2bpl/jar2bpl_test/regression/false_positives/fp16/FalsePositive16.java",68,7,68,14 } { :clone } { :comment "thenblock" } true;
+        goto block15;
+    } else {
+        assert { :sourceloc "/Users/schaef/git/jar2bpl/jar2bpl_test/regression/false_positives/fp16/FalsePositive16.java",68,7,68,14 } { :clone } { :comment "elseblock" } true;
+    }
+    assert { :sourceloc "/Users/schaef/git/jar2bpl/jar2bpl_test/regression/false_positives/fp16/FalsePositive16.java",68,7,68,14 } true;
+    goto block16;
+  block16:
+    assert { :sourceloc "/Users/schaef/git/jar2bpl/jar2bpl_test/regression/false_positives/fp16/FalsePositive16.java",68,19,68,33 } true;
+    if (truthValue32 == 0) {
+        assert { :sourceloc "/Users/schaef/git/jar2bpl/jar2bpl_test/regression/false_positives/fp16/FalsePositive16.java",68,19,68,33 } { :clone } { :comment "thenblock" } true;
+        goto block17;
+    } else {
+        assert { :sourceloc "/Users/schaef/git/jar2bpl/jar2bpl_test/regression/false_positives/fp16/FalsePositive16.java",68,19,68,33 } { :clone } { :comment "elseblock" } true;
+    }
+    assert { :sourceloc "/Users/schaef/git/jar2bpl/jar2bpl_test/regression/false_positives/fp16/FalsePositive16.java",68,19,68,33 } true;
+    goto block15;
+  block17:
+    assert { :sourceloc "/Users/schaef/git/jar2bpl/jar2bpl_test/regression/false_positives/fp16/FalsePositive16.java",69,4,69,10 } true;
+    return;
+  block15:
+    assert { :sourceloc "/Users/schaef/git/jar2bpl/jar2bpl_test/regression/false_positives/fp16/FalsePositive16.java",70,14,70,21 } true;
+    if (notEqual33 == 0) {
+        assert { :sourceloc "/Users/schaef/git/jar2bpl/jar2bpl_test/regression/false_positives/fp16/FalsePositive16.java",70,14,70,21 } { :clone } { :comment "thenblock" } true;
+        goto block18;
+    } else {
+        assert { :sourceloc "/Users/schaef/git/jar2bpl/jar2bpl_test/regression/false_positives/fp16/FalsePositive16.java",70,14,70,21 } { :clone } { :comment "elseblock" } true;
+    }
+    assert { :sourceloc "/Users/schaef/git/jar2bpl/jar2bpl_test/regression/false_positives/fp16/FalsePositive16.java",70,14,70,21 } true;
+    goto block19;
+  block19:
+    assert { :sourceloc "/Users/schaef/git/jar2bpl/jar2bpl_test/regression/false_positives/fp16/FalsePositive16.java",70,26,70,40 } true;
+    if (truthValue32 == 1) {
+        assert { :sourceloc "/Users/schaef/git/jar2bpl/jar2bpl_test/regression/false_positives/fp16/FalsePositive16.java",70,26,70,40 } { :clone } { :comment "thenblock" } true;
+        goto block20;
+    } else {
+        assert { :sourceloc "/Users/schaef/git/jar2bpl/jar2bpl_test/regression/false_positives/fp16/FalsePositive16.java",70,26,70,40 } { :clone } { :comment "elseblock" } true;
+    }
+    assert { :sourceloc "/Users/schaef/git/jar2bpl/jar2bpl_test/regression/false_positives/fp16/FalsePositive16.java",70,26,70,40 } true;
+    goto block18;
+  block20:
+    assert { :sourceloc "/Users/schaef/git/jar2bpl/jar2bpl_test/regression/false_positives/fp16/FalsePositive16.java",72,4,72,10 } true;
+    return;
+  block18:
+    assert { :sourceloc "/Users/schaef/git/jar2bpl/jar2bpl_test/regression/false_positives/fp16/FalsePositive16.java",73,15,73,22 } true;
+    if (notEqual33 == 0) {
+        assert { :sourceloc "/Users/schaef/git/jar2bpl/jar2bpl_test/regression/false_positives/fp16/FalsePositive16.java",73,15,73,22 } { :clone } { :comment "thenblock" } true;
+        goto block21;
+    } else {
+        assert { :sourceloc "/Users/schaef/git/jar2bpl/jar2bpl_test/regression/false_positives/fp16/FalsePositive16.java",73,15,73,22 } { :clone } { :comment "elseblock" } true;
+    }
+    assert { :sourceloc "/Users/schaef/git/jar2bpl/jar2bpl_test/regression/false_positives/fp16/FalsePositive16.java",73,15,73,22 } true;
+    goto block22;
+  block21:
+    assert { :sourceloc "/Users/schaef/git/jar2bpl/jar2bpl_test/regression/false_positives/fp16/FalsePositive16.java",73,27,73,41 } true;
+    if (truthValue32 == 0) {
+        assert { :sourceloc "/Users/schaef/git/jar2bpl/jar2bpl_test/regression/false_positives/fp16/FalsePositive16.java",73,27,73,41 } { :clone } { :comment "thenblock" } true;
+        goto block23;
+    } else {
+        assert { :sourceloc "/Users/schaef/git/jar2bpl/jar2bpl_test/regression/false_positives/fp16/FalsePositive16.java",73,27,73,41 } { :clone } { :comment "elseblock" } true;
+    }
+    assert { :sourceloc "/Users/schaef/git/jar2bpl/jar2bpl_test/regression/false_positives/fp16/FalsePositive16.java",73,27,73,41 } true;
+    goto block22;
+  block23:
+    assert { :sourceloc "/Users/schaef/git/jar2bpl/jar2bpl_test/regression/false_positives/fp16/FalsePositive16.java",74,4,74,10 } true;
+    return;
+  block22:
+    assert { :sourceloc "/Users/schaef/git/jar2bpl/jar2bpl_test/regression/false_positives/fp16/FalsePositive16.java",75,15,75,22 } true;
+    if (notEqual33 == 0) {
+        assert { :sourceloc "/Users/schaef/git/jar2bpl/jar2bpl_test/regression/false_positives/fp16/FalsePositive16.java",75,15,75,22 } { :clone } { :comment "thenblock" } true;
+        goto block24;
+    } else {
+        assert { :sourceloc "/Users/schaef/git/jar2bpl/jar2bpl_test/regression/false_positives/fp16/FalsePositive16.java",75,15,75,22 } { :clone } { :comment "elseblock" } true;
+    }
+    assert { :sourceloc "/Users/schaef/git/jar2bpl/jar2bpl_test/regression/false_positives/fp16/FalsePositive16.java",75,15,75,22 } true;
+    goto block25;
+  block24:
+    assert { :sourceloc "/Users/schaef/git/jar2bpl/jar2bpl_test/regression/false_positives/fp16/FalsePositive16.java",75,27,75,41 } true;
+    if (truthValue32 == 1) {
+        assert { :sourceloc "/Users/schaef/git/jar2bpl/jar2bpl_test/regression/false_positives/fp16/FalsePositive16.java",75,27,75,41 } { :clone } { :comment "thenblock" } true;
+        goto block26;
+    } else {
+        assert { :sourceloc "/Users/schaef/git/jar2bpl/jar2bpl_test/regression/false_positives/fp16/FalsePositive16.java",75,27,75,41 } { :clone } { :comment "elseblock" } true;
+    }
+    assert { :sourceloc "/Users/schaef/git/jar2bpl/jar2bpl_test/regression/false_positives/fp16/FalsePositive16.java",75,27,75,41 } true;
+    goto block25;
+  block26:
+    assert { :sourceloc "/Users/schaef/git/jar2bpl/jar2bpl_test/regression/false_positives/fp16/FalsePositive16.java",76,4,76,10 } true;
+    return;
+  block25:
+    assert { :sourceloc "/Users/schaef/git/jar2bpl/jar2bpl_test/regression/false_positives/fp16/FalsePositive16.java",78,4,78,32 } true;
+    call $fakelocal_0 := $new(java.lang.RuntimeException);
+    temp$034 := $fakelocal_0;
+    assert { :sourceloc "/Users/schaef/git/jar2bpl/jar2bpl_test/regression/false_positives/fp16/FalsePositive16.java",78,10,78,31 } true;
+    call $exception := void$java.lang.RuntimeException$$la$init$ra$$922(temp$034);
+    assert { :sourceloc "/Users/schaef/git/jar2bpl/jar2bpl_test/regression/false_positives/fp16/FalsePositive16.java",78,10,78,31 } true;
+    $exception := temp$034;
+    return;
+}
+
+
+implementation int$FalsePositive16$decisions$1895($this:ref, $in_parameter__0:int, $in_parameter__1:int) returns ($return:int, $exception:ref){
+    
+var temp$139 : int;    
+var lowercheck36 : int;    
+var temp$240 : int;    
+var temp$038 : int;    
+var uppercheck37 : int;    
+var temp$341 : int;    
+var this35 : ref;
+    assume { :sourceloc "/Users/schaef/git/jar2bpl/jar2bpl_test/regression/false_positives/fp16/FalsePositive16.java",-1,-1,-1,-1 } $this != $null;
+    assert { :sourceloc "/Users/schaef/git/jar2bpl/jar2bpl_test/regression/false_positives/fp16/FalsePositive16.java",82,2,87,2 } true;
+    this35 := $this;
+    assert { :sourceloc "/Users/schaef/git/jar2bpl/jar2bpl_test/regression/false_positives/fp16/FalsePositive16.java",82,23,82,40 } true;
+    lowercheck36 := $in_parameter__0;
+    assert { :sourceloc "/Users/schaef/git/jar2bpl/jar2bpl_test/regression/false_positives/fp16/FalsePositive16.java",82,43,82,60 } true;
+    uppercheck37 := $in_parameter__1;
+    assert { :sourceloc "/Users/schaef/git/jar2bpl/jar2bpl_test/regression/false_positives/fp16/FalsePositive16.java",83,13,83,22 } true;
+    if (lowercheck36 == 0) {
+        assert { :sourceloc "/Users/schaef/git/jar2bpl/jar2bpl_test/regression/false_positives/fp16/FalsePositive16.java",83,13,83,22 } { :clone } { :comment "thenblock" } true;
+        goto block27;
+    } else {
+        assert { :sourceloc "/Users/schaef/git/jar2bpl/jar2bpl_test/regression/false_positives/fp16/FalsePositive16.java",83,13,83,22 } { :clone } { :comment "elseblock" } true;
+    }
+    assert { :sourceloc "/Users/schaef/git/jar2bpl/jar2bpl_test/regression/false_positives/fp16/FalsePositive16.java",83,13,83,22 } true;
+    goto block28;
+  block28:
+    assert { :sourceloc "/Users/schaef/git/jar2bpl/jar2bpl_test/regression/false_positives/fp16/FalsePositive16.java",83,27,83,36 } true;
+    if (uppercheck37 == 0) {
+        assert { :sourceloc "/Users/schaef/git/jar2bpl/jar2bpl_test/regression/false_positives/fp16/FalsePositive16.java",83,27,83,36 } { :clone } { :comment "thenblock" } true;
+        goto block27;
+    } else {
+        assert { :sourceloc "/Users/schaef/git/jar2bpl/jar2bpl_test/regression/false_positives/fp16/FalsePositive16.java",83,27,83,36 } { :clone } { :comment "elseblock" } true;
+    }
+    assert { :sourceloc "/Users/schaef/git/jar2bpl/jar2bpl_test/regression/false_positives/fp16/FalsePositive16.java",83,27,83,36 } true;
+    goto block29;
+  block29:
+    assert { :sourceloc "/Users/schaef/git/jar2bpl/jar2bpl_test/regression/false_positives/fp16/FalsePositive16.java",83,27,83,36 } true;
+    temp$038 := 0;
+    assert { :sourceloc "/Users/schaef/git/jar2bpl/jar2bpl_test/regression/false_positives/fp16/FalsePositive16.java",83,39,83,47 } true;
+    $return := temp$038;
+    return;
+  block27:
+    assert { :sourceloc "/Users/schaef/git/jar2bpl/jar2bpl_test/regression/false_positives/fp16/FalsePositive16.java",84,13,84,22 } true;
+    if (lowercheck36 == 0) {
+        assert { :sourceloc "/Users/schaef/git/jar2bpl/jar2bpl_test/regression/false_positives/fp16/FalsePositive16.java",84,13,84,22 } { :clone } { :comment "thenblock" } true;
+        goto block30;
+    } else {
+        assert { :sourceloc "/Users/schaef/git/jar2bpl/jar2bpl_test/regression/false_positives/fp16/FalsePositive16.java",84,13,84,22 } { :clone } { :comment "elseblock" } true;
+    }
+    assert { :sourceloc "/Users/schaef/git/jar2bpl/jar2bpl_test/regression/false_positives/fp16/FalsePositive16.java",84,13,84,22 } true;
+    goto block31;
+  block31:
+    assert { :sourceloc "/Users/schaef/git/jar2bpl/jar2bpl_test/regression/false_positives/fp16/FalsePositive16.java",84,28,84,37 } true;
+    if (uppercheck37 == 0) {
+        assert { :sourceloc "/Users/schaef/git/jar2bpl/jar2bpl_test/regression/false_positives/fp16/FalsePositive16.java",84,28,84,37 } { :clone } { :comment "thenblock" } true;
+        goto block32;
+    } else {
+        assert { :sourceloc "/Users/schaef/git/jar2bpl/jar2bpl_test/regression/false_positives/fp16/FalsePositive16.java",84,28,84,37 } { :clone } { :comment "elseblock" } true;
+    }
+    assert { :sourceloc "/Users/schaef/git/jar2bpl/jar2bpl_test/regression/false_positives/fp16/FalsePositive16.java",84,28,84,37 } true;
+    goto block30;
+  block32:
+    assert { :sourceloc "/Users/schaef/git/jar2bpl/jar2bpl_test/regression/false_positives/fp16/FalsePositive16.java",84,28,84,37 } true;
+    temp$139 := 1;
+    assert { :sourceloc "/Users/schaef/git/jar2bpl/jar2bpl_test/regression/false_positives/fp16/FalsePositive16.java",84,40,84,48 } true;
+    $return := temp$139;
+    return;
+  block30:
+    assert { :sourceloc "/Users/schaef/git/jar2bpl/jar2bpl_test/regression/false_positives/fp16/FalsePositive16.java",85,19,85,28 } true;
+    if (lowercheck36 == 0) {
+        assert { :sourceloc "/Users/schaef/git/jar2bpl/jar2bpl_test/regression/false_positives/fp16/FalsePositive16.java",85,19,85,28 } { :clone } { :comment "thenblock" } true;
+        goto block33;
+    } else {
+        assert { :sourceloc "/Users/schaef/git/jar2bpl/jar2bpl_test/regression/false_positives/fp16/FalsePositive16.java",85,19,85,28 } { :clone } { :comment "elseblock" } true;
+    }
+    assert { :sourceloc "/Users/schaef/git/jar2bpl/jar2bpl_test/regression/false_positives/fp16/FalsePositive16.java",85,19,85,28 } true;
+    goto block34;
+  block33:
+    assert { :sourceloc "/Users/schaef/git/jar2bpl/jar2bpl_test/regression/false_positives/fp16/FalsePositive16.java",85,33,85,42 } true;
+    if (uppercheck37 == 0) {
+        assert { :sourceloc "/Users/schaef/git/jar2bpl/jar2bpl_test/regression/false_positives/fp16/FalsePositive16.java",85,33,85,42 } { :clone } { :comment "thenblock" } true;
+        goto block34;
+    } else {
+        assert { :sourceloc "/Users/schaef/git/jar2bpl/jar2bpl_test/regression/false_positives/fp16/FalsePositive16.java",85,33,85,42 } { :clone } { :comment "elseblock" } true;
+    }
+    assert { :sourceloc "/Users/schaef/git/jar2bpl/jar2bpl_test/regression/false_positives/fp16/FalsePositive16.java",85,33,85,42 } true;
+    goto block35;
+  block35:
+    assert { :sourceloc "/Users/schaef/git/jar2bpl/jar2bpl_test/regression/false_positives/fp16/FalsePositive16.java",85,33,85,42 } true;
+    temp$240 := 2;
+    assert { :sourceloc "/Users/schaef/git/jar2bpl/jar2bpl_test/regression/false_positives/fp16/FalsePositive16.java",85,45,85,53 } true;
+    $return := temp$240;
+    return;
+  block34:
+    assert { :sourceloc "/Users/schaef/git/jar2bpl/jar2bpl_test/regression/false_positives/fp16/FalsePositive16.java",85,45,85,53 } true;
+    temp$341 := 3;
+    assert { :sourceloc "/Users/schaef/git/jar2bpl/jar2bpl_test/regression/false_positives/fp16/FalsePositive16.java",86,14,86,22 } true;
+    $return := temp$341;
+    return;
+}
+
+
+implementation void$FalsePositive16$$la$init$ra$$1896($this:ref) returns ($exception:ref){
+    
+var this42 : ref;
+    assume { :sourceloc "/Users/schaef/git/jar2bpl/jar2bpl_test/regression/false_positives/fp16/FalsePositive16.java",-1,-1,-1,-1 } $this != $null;
+    assert { :sourceloc "/Users/schaef/git/jar2bpl/jar2bpl_test/regression/false_positives/fp16/FalsePositive16.java",5,-1,-1,-1 } true;
+    this42 := $this;
+    assert { :sourceloc "/Users/schaef/git/jar2bpl/jar2bpl_test/regression/false_positives/fp16/FalsePositive16.java",5,-1,-1,-1 } true;
+    call $exception := void$java.lang.Object$$la$init$ra$$38(this42);
+    assert { :sourceloc "/Users/schaef/git/jar2bpl/jar2bpl_test/regression/false_positives/fp16/FalsePositive16.java",5,-1,-1,-1 } true;
+    return;
+}
 
 
